case_studies/tests/output/tests/proofs/proof_traits_foo_call_foobar.v
@@ -17,6 +17,7 @@ Proof.
   all: print_remaining_goal.
   Unshelve. all: sidecond_solver.
   Unshelve. all: sidecond_hammer.
+
   Unshelve. all: print_remaining_sidecond.
 Qed.
 End proof.
